

MIT 18.03 Linear Operator

Nilangshu Sarkar

December 2025

Part 1

3.

Problem 3: Find a particular solution to the DE

$$y^{(4)} - 2y'' + y = xe^x$$

Let

$$D = \frac{d}{dx} \implies Dy = \frac{dy}{dx} = y' \implies D^2y = y'' \& D^4y = y''''$$

So the given Equation becomes

$$(D^4 - 2D^2 + 1)y = xe^x$$

Let

$$(D^4 - 2D^2 + 1) = L(D) \implies L(D)y = xe^x$$

Therefore Particular Solution is given by

$$\begin{aligned} y_P &= \left\{ \frac{1}{L(D)} \right\} (xe^x) = e^x \left\{ \frac{1}{L(D+1)} \right\} (x) \\ &= e^x \left\{ \frac{1}{(D+1)^4 - 2(D+1)^2 + 1} \right\} (x) = e^x \left\{ \frac{1}{((D+1)^2 - 1)^2} \right\} (x) \\ &= e^x \left\{ (D^2 + 2D)^{-2} \right\} (x) \end{aligned}$$

Let

$$u = \left\{ (D^2 + 2D)^{-2} \right\} (x) \implies \left\{ (D^2 + 2D)^2 \right\} u = x$$

For $(D^2 + 2D)$ we can set our Solution as $(Ax^2 + Bx + C)$
 Here $(D^2 + 2D)$ applied twice.
 So the expression of u will be of the form

$$u = (1 + x)(Ax^2 + Bx + C) = (A)x^3 + (A + B)x^2 + (B + C)x + (C)$$

Therefore we get

$$\begin{aligned} Du &= (3A)x^2 + (2A + 2B)x + (B + C) \\ \implies 2Du &= (6A)x^2 + (4A + 4B)x + (2B + 2C) \\ D^2u &= (6A)x + (2A + 2B) \end{aligned}$$

Let

$$v = (D^2 + 2D)u = (6A)x^2 + (10A + 4B)x + (2A + 4B + 2C)$$

So

$$\begin{aligned} Dv &= (12A)x + (10A + 4B) \\ \implies 2Dv &= (24A)x + (20A + 8B) \\ D^2v &= (12A) \end{aligned}$$

This gives us

$$(D^2 + 2D)v = (24A)x + (32A + 8B)$$

But

$$\begin{aligned} (D^2 + 2D)v &= x \\ \implies (24A)x + (32A + 8B) &= x \\ \implies A &= \frac{1}{24} \text{ and } B = -\frac{1}{6} \end{aligned}$$

Since C is arbitrary, we can set $C = 0$ for a Particular solution. In case any I.C.s were given, we could formulate a General Solution where the C.F. could have compensated for the C . So setting $C = 0$ will cause no trouble at all.

Hence,

$$u = (1 + x)\left(\frac{x^2}{24} - \frac{x}{6}\right)$$

Therefore, The Particular Solution is given by

$$y_P = e^x(1 + x)\left(\frac{x^2}{24} - \frac{x}{6}\right)$$